![[Hochschule/Module/Lineare Algebra/Ãœbung/LA_Aufgabensammlung_02.excalidraw.md#^area=1gvu9ZC31hRMwJxPXHDum|100%]]

(1)
$f: \mathbb{R}^{2} \to \mathbb{R}^{2}$
$f(x) =\lambda x,\lambda \in \mathbb{R}$

$x=\begin{pmatrix}x_{1} \\ x_{2}\end{pmatrix}$

$A_{f} =\lambda (f(e_{1}^{2}), f(e_{2}^{2}))$
$=\lambda (f(\begin{pmatrix}1  \\ 0\end{pmatrix}), f(\begin{pmatrix}0  \\ 1\end{pmatrix}))$
$=\lambda (\begin{pmatrix}1 \\ 0\end{pmatrix}, \begin{pmatrix}0 \\ 1\end{pmatrix})$
$=\lambda (\begin{pmatrix}1  & 0 \\ 0  &  1\end{pmatrix})$
$=\begin{pmatrix}\lambda & 0 \\ 0 &\lambda\end{pmatrix}$

(2)
$g: \mathbb{R}^{2}\to\mathbb{R}^{3}$
$g(x)=g(\begin{pmatrix}x_{1} \\ x_{2}\end{pmatrix})=\begin{pmatrix}x_{2} \\ x_{1} \\ x_{1}+x_{2}\end{pmatrix}$

$A_{f}=\begin{pmatrix}0 & 1 \\ 1 & 0 \\ 1 & 1\end{pmatrix}$

(3)
$g \circ f: \mathbb{R}^{2}\to\mathbb{R}^{3}$

$g(f(x))=g(\lambda x)=\lambda g(x)=\lambda \begin{pmatrix}0 & 1 \\ 1 & 0 \\ 1 & 1\end{pmatrix}=\begin{pmatrix}0 & \lambda \\ \lambda & 0 \\ \lambda & \lambda\end{pmatrix}$
